docs/03-formal-verification/easycrypt/games/GameMSHopComposition.ec
@@ -1,7 +1,7 @@
 require import AllCore List.
 require import StdOrder.
 (*---*) import RealOrder.
-require import QssmTypes Algebra Simulator FS TrueClause Comparison ComparisonTypes ComparisonDigests ComparisonPayloads ComparisonCoupling ComparisonCouplingTypes ComparisonCouplingAxioms ComparisonCouplingTheorem ComparisonTheorem.
+require import QssmTypes Algebra Simulator FS TrueClause Comparison ComparisonTypes ComparisonDigests ComparisonPayload ComparisonCoupling ComparisonCouplingTypes ComparisonCouplingAxioms ComparisonCouplingTheorem ComparisonTheorem.
 require import SourceDistributions SourceTheorem MS LESurface LEModel.
 require import GameTypes GameViews GameAdvantage GameMSHopTypes GameMSHopTransitions.
 
