docs/03-formal-verification/easycrypt/ms/comparison/ComparisonCouplingSchedule.ec
@@ -1,0 +1,175 @@
+require import AllCore List Distr.
+require import Algebra QssmTypes FS SchnorrBranch TrueClause BitnessOne.
+require import ComparisonTypes ComparisonDigests ComparisonPayload ComparisonCouplingTypes
+  ComparisonCouplingAxioms ComparisonCouplingMarginals.
+
+lemma A_ms3c_payload_support_coupling_from_components :
+  forall (x : ms_public_input) (s : seed),
+    ms3c_ax_payload_public_fields_match x s =>
+    ms3c_ax_payload_challenge_shares_match x s =>
+    ms3c_ax_payload_challenge_share_consistency x s =>
+    ms3c_ax_payload_false_clauses_simulated x s =>
+    ms3c_ax_payload_true_clause_simulated x s =>
+    ms3c_ax_payload_support_coupling x s.
+proof.
+move=> x s Hpub Hshr Hcons Hfalse Htrue.
+rewrite /ms3c_ax_payload_support_coupling.
+split.
+  have Hll_sim := L_ms3c_sim_comparison_payload_law_lossless x s.
+  have Heq := L_ms3c_coupling_real_projection_eq_payload x s Hll_sim.
+  apply (L_ms3c_coupling_real_marginal_eq x s).
+    by move=> pr; rewrite Heq.
+  by move=> pr Hpr; rewrite -Heq.
+split.
+  have Hll_real := L_ms3c_real_comparison_payload_law_lossless x.
+  have Heq := L_ms3c_coupling_sim_projection_eq_payload x s Hll_real.
+  apply (L_ms3c_coupling_sim_marginal_eq x s).
+    by move=> ps; rewrite Heq.
+  by move=> ps Hps; rewrite -Heq.
+exact (A_ms3c_coupling_pair_relation x s Hpub Hshr Hcons Hfalse Htrue).
+qed.
+
+lemma L_ms3c_payload_eq_of_coupled
+  (pr : ms3c_real_comparison_payload) (ps : ms3c_sim_comparison_payload) :
+  ms3c_real_sim_payload_coupled pr ps =>
+  pr = ps.
+proof.
+case: pr=> tr fr atr afr str sfr gcr qdr pcr.
+case: ps=> ts fs ats afs sts sfs gcs qds pcs /=.
+move=> [Hpub [Hshr _]].
+move: Hpub=> [Htr [Hfr [Hatr [Hafr [Hqd [Hgc Hpc]]]]]].
+move: Hshr=> [Hstr Hsfr].
+by subst.
+qed.
+
+lemma L_ms3c_coupling_fst_snd_eq_from_pair_relation
+  (x : ms_public_input) (s : seed) :
+  ms3c_ax_payload_coupling_pair_relation x s =>
+  d_ms3c_coupling_real_projection x s = d_ms3c_coupling_sim_projection x s.
+proof.
+move=> Hpair.
+rewrite /d_ms3c_coupling_real_projection /d_ms3c_coupling_sim_projection.
+apply eq_dmap_in.
+move=> [] pr ps Hmem.
+have Hcpl := Hpair pr ps Hmem.
+exact (L_ms3c_payload_eq_of_coupled pr ps Hcpl).
+qed.
+
+lemma A_ms3c_payload_schedule_eq_from_coupling
+  (x : ms_public_input) (s : seed) :
+  ms3c_ax_payload_support_coupling x s =>
+  d_ms3c_real_comparison_payload x = d_ms3c_sim_comparison_payload x s.
+proof.
+move=> [Hre [Hsi Hpr]].
+have HeqJ := L_ms3c_coupling_fst_snd_eq_from_pair_relation x s Hpr.
+by rewrite -Hre HeqJ Hsi.
+qed.
+
+lemma L_ms3c_payload_announcement_digests_preserved_from_public_fields
+  (x : ms_public_input) (s : seed) :
+  ms3c_ax_payload_public_fields_match x s =>
+  ms3c_ax_payload_announcement_digests_preserved x s.
+proof.
+move=> Hpub pr ps Hpr Hps.
+have Hm := Hpub pr ps Hpr Hps.
+move: Hm => [_ [_ [Hann_t [Hann_f _]]]].
+by rewrite /ms3c_clause_ann_digests_from_surface /ms3c_make_real_clause_surface
+  /ms3c_make_sim_clause_surface /ms3c_make_clause_surface
+  /ms3c_digest_true_announcement /ms3c_digest_false_announcements /= Hann_t Hann_f.
+qed.
+
+lemma L_ms3c_payload_announcements_match_shape_from_ann_hook
+  (x : ms_public_input) (s : seed) :
+  (forall (pr : ms3c_real_comparison_payload),
+    ms3c_real_payload_on_support x pr =>
+    ms_comparison_clause_simulatable (ms3c_make_real_clause_surface pr)) =>
+  (forall (ps : ms3c_sim_comparison_payload),
+    ms3c_sim_payload_on_support x s ps =>
+    ms_comparison_clause_simulatable (ms3c_make_sim_clause_surface ps)) =>
+  ms3c_ax_payload_announcements_match_shape x s.
+proof.
+move=> _ _.
+exact (L_ms3c_ax_payload_announcements_match_shape_total x s).
+qed.
+
+lemma L_ms3c_payload_challenge_share_consistency_from_sum_hook
+  (x : ms_public_input) (s : seed) :
+  ms3c_clause_challenge_shares_sum x s =>
+  (forall (pr : ms3c_real_comparison_payload),
+    ms3c_real_payload_on_support x pr =>
+    ms_comparison_clause_simulatable (ms3c_make_real_clause_surface pr)) =>
+  (forall (ps : ms3c_sim_comparison_payload),
+    ms3c_sim_payload_on_support x s ps =>
+    ms_comparison_clause_simulatable (ms3c_make_sim_clause_surface ps)) =>
+  ms3c_ax_payload_challenge_share_consistency x s.
+proof.
+move=> Hsum Hreal Hsim.
+rewrite /ms3c_ax_payload_challenge_share_consistency /ms3c_payload_programmed_challenge_matches_global.
+split.
+  move=> pr Hpr.
+  by apply (Hsum (ms3c_make_real_clause_surface pr) (Hreal pr Hpr)).
+move=> ps Hps.
+by apply (Hsum (ms3c_make_sim_clause_surface ps) (Hsim ps Hps)).
+qed.
+
+lemma L_ms3c_payload_true_clause_simulated_from_true_hook
+  (x : ms_public_input) (s : seed) :
+  ms3c_true_clause_schnorr_from_blinder x s =>
+  ms3c_ax_payload_true_clause_simulated x s.
+proof.
+move=> Htrue.
+rewrite /ms3c_ax_payload_true_clause_simulated.
+split.
+  move=> vb tb p r pr _ Hbl Hpos.
+  by apply (A_ms3c_true_clause_from_ms3b_and_schnorr x s Htrue vb tb p r (ms3c_make_real_clause_surface pr) Hbl Hpos).
+move=> vb tb p r ps _ Hbl Hpos.
+by apply (A_ms3c_true_clause_from_ms3b_and_schnorr x s Htrue vb tb p r (ms3c_make_sim_clause_surface ps) Hbl Hpos).
+qed.
+
+lemma A_ms3c_payload_schedule_equiv :
+  forall (x : ms_public_input) (s : seed),
+    ms3c_comparison_query_digest_ann_only x s =>
+    ms3c_comparison_global_programmable_under_A2 x s =>
+    ms3c_false_clauses_simulator_generated x s =>
+    ms3c_true_clause_schnorr_from_blinder x s =>
+    ms3c_clause_challenge_shares_sum x s =>
+    d_ms3c_real_comparison_payload x = d_ms3c_sim_comparison_payload x s.
+proof.
+move=> x s Hann Ha2 Hfalse Htrue Hsum.
+have Hreal : forall (pr : ms3c_real_comparison_payload),
+    ms3c_real_payload_on_support x pr =>
+    ms_comparison_clause_simulatable (ms3c_make_real_clause_surface pr).
+  by move=> pr Hpr; apply (L_ms3c_real_payload_support_simulatable x pr Hpr).
+have Hsim : forall (ps : ms3c_sim_comparison_payload),
+    ms3c_sim_payload_on_support x s ps =>
+    ms_comparison_clause_simulatable (ms3c_make_sim_clause_surface ps).
+  by move=> ps Hps; apply (L_ms3c_sim_payload_support_simulatable x s ps Hps).
+have Hpub := A_ms3c_payload_public_fields_match x s Hann Ha2 Hfalse Htrue Hsum.
+have Hshr := A_ms3c_payload_challenge_shares_match x s Hann Ha2 Hfalse Htrue Hsum.
+have Hcons :=
+  L_ms3c_payload_challenge_share_consistency_from_sum_hook x s Hsum Hreal Hsim.
+have Hfalse_nt := A_ms3c_false_clauses_hook_implies_schedule_nontrivial x s Hfalse.
+have Hfalse_payload := A_ms3c_false_clause_simulation x s Hfalse_nt.
+have Htrue_payload := L_ms3c_payload_true_clause_simulated_from_true_hook x s Htrue.
+have Hcpl :=
+  A_ms3c_payload_support_coupling_from_components x s
+    Hpub Hshr Hcons Hfalse_payload Htrue_payload.
+exact (A_ms3c_payload_schedule_eq_from_coupling x s Hcpl).
+qed.
+
+lemma A_ms3c_comparison_schedule_equiv :
+  forall (x : ms_public_input) (s : seed),
+    ms3c_comparison_query_digest_ann_only x s =>
+    ms3c_comparison_global_programmable_under_A2 x s =>
+    ms3c_false_clauses_simulator_generated x s =>
+    ms3c_true_clause_schnorr_from_blinder x s =>
+    ms3c_clause_challenge_shares_sum x s =>
+    d_ms3c_real_comparison_schedule x = d_ms3c_sim_comparison_schedule x s.
+proof.
+move=> x s Hann Ha2 Hfalse Htrue Hsum.
+have Hp := A_ms3c_payload_schedule_equiv x s Hann Ha2 Hfalse Htrue Hsum.
+rewrite /d_ms3c_real_comparison_schedule /d_ms3c_sim_comparison_schedule
+  /ms3c_make_real_clause_surface /ms3c_make_sim_clause_surface.
+exact (qssm_dmap_congr (d_ms3c_real_comparison_payload x) (d_ms3c_sim_comparison_payload x s)
+  ms3c_make_clause_surface Hp).
+qed.
