docs/03-formal-verification/easycrypt/ms/comparison/ComparisonPayloadFalseClause.ec
@@ -1,0 +1,113 @@
+require import AllCore List Distr.
+require import Algebra QssmTypes FS SchnorrBranch TrueClause BitnessOne.
+require import ComparisonTypes ComparisonDigests ComparisonPayloadTypes
+  ComparisonPayloadSeeds ComparisonPayloadSupport.
+
+(* False-branch width, simulation on support, and simulatable packaging. *)
+
+axiom A_ms3c_real_constructor_false_index_nonempty :
+  forall (x : ms_public_input) (sr : ms3c_real_payload_seed),
+    0 < size (ms3c_real_payload_from_seed x sr).`mscp_false_clause_ixs.
+
+axiom A_ms3c_sim_constructor_false_index_nonempty :
+  forall (x : ms_public_input) (s : seed) (ss : ms3c_sim_payload_seed),
+    0 < size (ms3c_sim_payload_from_seed x s ss).`mscp_false_clause_ixs.
+
+lemma A_ms3c_real_seed_false_index_nonempty :
+  forall (x : ms_public_input) (sr : ms3c_real_payload_seed),
+    0 < size (ms3c_real_payload_from_seed x sr).`mscp_false_clause_ixs.
+proof.
+by move=> x sr; exact (A_ms3c_real_constructor_false_index_nonempty x sr).
+qed.
+
+lemma A_ms3c_sim_seed_false_index_nonempty :
+  forall (x : ms_public_input) (s : seed) (ss : ms3c_sim_payload_seed),
+    0 < size (ms3c_sim_payload_from_seed x s ss).`mscp_false_clause_ixs.
+proof.
+by move=> x s ss; exact (A_ms3c_sim_constructor_false_index_nonempty x s ss).
+qed.
+
+lemma A_ms3c_real_seed_false_clause_nonempty :
+  forall (x : ms_public_input) (sr : ms3c_real_payload_seed),
+    0 < size (ms3c_real_payload_from_seed x sr).`mscp_ann_false.
+proof.
+move=> x sr.
+have Hix_pos := A_ms3c_real_seed_false_index_nonempty x sr.
+have [_ Hshape] := A_ms3c_real_seed_index_shape_valid x sr.
+rewrite Hshape.
+exact Hix_pos.
+qed.
+
+lemma A_ms3c_sim_seed_false_clause_nonempty :
+  forall (x : ms_public_input) (s : seed) (ss : ms3c_sim_payload_seed),
+    0 < size (ms3c_sim_payload_from_seed x s ss).`mscp_ann_false.
+proof.
+move=> x s ss.
+have Hix_pos := A_ms3c_sim_seed_false_index_nonempty x s ss.
+have [_ Hshape] := A_ms3c_sim_seed_index_shape_valid x s ss.
+rewrite Hshape.
+exact Hix_pos.
+qed.
+
+lemma A_ms3c_false_clauses_hook_implies_schedule_nontrivial :
+  forall (x : ms_public_input) (s : seed),
+    ms3c_false_clauses_simulator_generated x s =>
+    ms3c_false_clauses_payload_schedule_nontrivial x s.
+proof.
+move=> x s _.
+have Hll : is_lossless (d_ms3c_real_payload_seed x).
+  exact (L_ms3c_real_payload_seed_lossless x).
+have Hmu : mu (d_ms3c_real_payload_seed x) predT <> 0%r.
+  rewrite /is_lossless /weight in Hll.
+  by rewrite Hll.
+have [sr Hsr] : exists (sr : ms3c_real_payload_seed), sr \in d_ms3c_real_payload_seed x.
+  have [sr [Hsr _]] := neq0_mu (d_ms3c_real_payload_seed x) predT Hmu.
+  by exists sr.
+left.
+exists (ms3c_real_payload_from_seed x sr).
+split.
+  rewrite /ms3c_real_payload_on_support /d_ms3c_real_comparison_payload.
+  apply supp_dmap.
+  by exists sr.
+exact (A_ms3c_real_seed_false_clause_nonempty x sr).
+qed.
+
+axiom A_ms3c_false_clause_generation_on_support :
+  forall (x : ms_public_input) (s : seed),
+    ms3c_ax_payload_false_clauses_simulated x s.
+
+lemma A_ms3c_false_clause_simulation :
+  forall (x : ms_public_input) (s : seed),
+    ms3c_false_clauses_payload_schedule_nontrivial x s =>
+    ms3c_ax_payload_false_clauses_simulated x s.
+proof.
+by move=> x s _; exact (A_ms3c_false_clause_generation_on_support x s).
+qed.
+
+lemma L_ms_comparison_clause_simulatable_of_payload_length_index
+  (p : ms3c_comparison_clause_payload) :
+  ms3c_payload_length_index_shapes_ok p =>
+  ms_comparison_clause_simulatable (ms3c_make_clause_surface p).
+proof.
+move=> H.
+rewrite /ms_comparison_clause_simulatable /ms3c_make_clause_surface /=.
+by [].
+qed.
+
+lemma L_ms3c_real_payload_support_simulatable (x : ms_public_input) (pr : ms3c_real_comparison_payload) :
+  ms3c_real_payload_on_support x pr =>
+  ms_comparison_clause_simulatable (ms3c_make_real_clause_surface pr).
+proof.
+move=> Hsup.
+apply (L_ms_comparison_clause_simulatable_of_payload_length_index pr).
+exact (A_ms3c_real_payload_support_length_index_shapes x pr Hsup).
+qed.
+
+lemma L_ms3c_sim_payload_support_simulatable (x : ms_public_input) (s : seed) (ps : ms3c_sim_comparison_payload) :
+  ms3c_sim_payload_on_support x s ps =>
+  ms_comparison_clause_simulatable (ms3c_make_sim_clause_surface ps).
+proof.
+move=> Hsup.
+apply (L_ms_comparison_clause_simulatable_of_payload_length_index ps).
+exact (A_ms3c_sim_payload_support_length_index_shapes x s ps Hsup).
+qed.
