docs/03-formal-verification/easycrypt/ms/source/SourcePublicFieldObligations.ec
@@ -1,0 +1,130 @@
+require import AllCore List Distr.
+require import QssmTypes FS SchnorrBranch BitnessOne BitnessVector.
+require import SourceTypes SourceConstructors SourceDistributions.
+require import SourceProgrammedObligations.
+
+(* Paired public-field seed axioms, `from_seed` lemmas, and payload-support programming. *)
+
+axiom A_ms3a_seed_pair_stmt_source_shared (x : ms_public_input) (s : seed) :
+  forall (sr : ms3a_real_payload_seed) (ss : ms3a_sim_payload_seed),
+    sr \in d_ms3a_real_payload_seed x =>
+    ss \in d_ms3a_sim_payload_seed x s =>
+    sr.`ms3rp_stmt = ss.`ms3sp_stmt.
+
+lemma A_ms3a_seed_pair_stmt_on_support (x : ms_public_input) (s : seed) :
+  forall (sr : ms3a_real_payload_seed) (ss : ms3a_sim_payload_seed),
+    sr \in d_ms3a_real_payload_seed x =>
+    ss \in d_ms3a_sim_payload_seed x s =>
+    (ms3a_real_payload_from_seed x sr).`ms3rp_stmt =
+      (ms3a_sim_payload_from_seed x s ss).`ms3sp_stmt.
+proof.
+move=> sr ss Hsr Hss.
+exact (ms3a_payload_pair_stmt_eq_from_seed_of_seed_stmt_eq x s sr ss
+  (A_ms3a_seed_pair_stmt_source_shared x s sr ss Hsr Hss)).
+qed.
+
+axiom A_ms3a_seed_pair_res_source_shared (x : ms_public_input) (s : seed) :
+  forall (sr : ms3a_real_payload_seed) (ss : ms3a_sim_payload_seed),
+    sr \in d_ms3a_real_payload_seed x =>
+    ss \in d_ms3a_sim_payload_seed x s =>
+    sr.`ms3rp_res = ss.`ms3sp_res.
+
+lemma A_ms3a_seed_pair_res_on_support (x : ms_public_input) (s : seed) :
+  forall (sr : ms3a_real_payload_seed) (ss : ms3a_sim_payload_seed),
+    sr \in d_ms3a_real_payload_seed x =>
+    ss \in d_ms3a_sim_payload_seed x s =>
+    (ms3a_real_payload_from_seed x sr).`ms3rp_res =
+      (ms3a_sim_payload_from_seed x s ss).`ms3sp_res.
+proof.
+move=> sr ss Hsr Hss.
+exact (ms3a_payload_pair_res_eq_from_seed_of_seed_res_eq x s sr ss
+  (A_ms3a_seed_pair_res_source_shared x s sr ss Hsr Hss)).
+qed.
+
+axiom A_ms3a_seed_pair_comparison_global_source_shared
+  (x : ms_public_input) (s : seed) :
+  forall (sr : ms3a_real_payload_seed) (ss : ms3a_sim_payload_seed),
+    sr \in d_ms3a_real_payload_seed x =>
+    ss \in d_ms3a_sim_payload_seed x s =>
+    sr.`ms3rp_comparison_global_challenge = ss.`ms3sp_comparison_global_challenge.
+
+lemma A_ms3a_seed_pair_comparison_global_on_support (x : ms_public_input) (s : seed) :
+  forall (sr : ms3a_real_payload_seed) (ss : ms3a_sim_payload_seed),
+    sr \in d_ms3a_real_payload_seed x =>
+    ss \in d_ms3a_sim_payload_seed x s =>
+    (ms3a_real_payload_from_seed x sr).`ms3rp_comparison_global_challenge =
+      (ms3a_sim_payload_from_seed x s ss).`ms3sp_comparison_global_challenge.
+proof.
+move=> sr ss Hsr Hss.
+exact (ms3a_payload_pair_comparison_global_challenge_eq_from_seed_of_seed_eq x s sr ss
+  (A_ms3a_seed_pair_comparison_global_source_shared x s sr ss Hsr Hss)).
+qed.
+
+axiom A_ms3a_seed_pair_bitness_globals_source_shared
+  (x : ms_public_input) (s : seed) :
+  forall (sr : ms3a_real_payload_seed) (ss : ms3a_sim_payload_seed),
+    sr \in d_ms3a_real_payload_seed x =>
+    ss \in d_ms3a_sim_payload_seed x s =>
+    sr.`ms3rp_bitness_global_challenges = ss.`ms3sp_bitness_global_challenges.
+
+lemma A_ms3a_seed_pair_bitness_globals_on_support (x : ms_public_input) (s : seed) :
+  forall (sr : ms3a_real_payload_seed) (ss : ms3a_sim_payload_seed),
+    sr \in d_ms3a_real_payload_seed x =>
+    ss \in d_ms3a_sim_payload_seed x s =>
+    (ms3a_real_payload_from_seed x sr).`ms3rp_bitness_global_challenges =
+      (ms3a_sim_payload_from_seed x s ss).`ms3sp_bitness_global_challenges.
+proof.
+move=> sr ss Hsr Hss.
+exact (ms3a_payload_pair_bitness_global_challenges_eq_from_seed_of_seed_eq x s sr ss
+  (A_ms3a_seed_pair_bitness_globals_source_shared x s sr ss Hsr Hss)).
+qed.
+
+lemma A_ms3a_seed_pair_public_fields_on_support
+  (x : ms_public_input) (s : seed) :
+  forall (sr : ms3a_real_payload_seed) (ss : ms3a_sim_payload_seed),
+    sr \in d_ms3a_real_payload_seed x =>
+    ss \in d_ms3a_sim_payload_seed x s =>
+    ms3a_payload_pair_public_fields_match
+      (ms3a_real_payload_from_seed x sr) (ms3a_sim_payload_from_seed x s ss).
+proof.
+move=> sr ss Hsr Hss.
+rewrite ms3a_real_payload_from_seed_def ms3a_sim_payload_from_seed_def.
+rewrite /ms3a_payload_pair_public_fields_match.
+split; first exact (A_ms3a_seed_pair_stmt_on_support x s sr ss Hsr Hss).
+split; first exact (A_ms3a_seed_pair_res_on_support x s sr ss Hsr Hss).
+split; first exact (A_ms3a_seed_pair_comparison_global_on_support x s sr ss Hsr Hss).
+exact (A_ms3a_seed_pair_bitness_globals_on_support x s sr ss Hsr Hss).
+qed.
+
+lemma ms3a_payload_real_support_programmed (x : ms_public_input) :
+  forall (p : ms3a_real_source_payload),
+    p \in d_ms3a_real_source_payload x => ms3a_real_payload_programmed_layer p.
+proof.
+move=> p Hp; move: Hp; rewrite /d_ms3a_real_source_payload => Hp.
+case/supp_dmap: Hp=> [sigma [Hsig Heq]].
+rewrite Heq; exact (A_ms3a_real_seed_programmed_on_support x sigma Hsig).
+qed.
+
+lemma ms3a_payload_sim_support_programmed (x : ms_public_input) (s : seed) :
+  forall (p : ms3a_sim_source_payload),
+    p \in d_ms3a_sim_source_payload x s => ms3a_sim_payload_programmed_layer p.
+proof.
+move=> p Hp; move: Hp; rewrite /d_ms3a_sim_source_payload => Hp.
+case/supp_dmap: Hp=> [sigma [Hsig Heq]].
+rewrite Heq; exact (A_ms3a_sim_seed_programmed_on_support x s sigma Hsig).
+qed.
+
+lemma ms3a_payload_pair_public_fields_on_support
+  (x : ms_public_input) (s : seed) :
+  forall (pr : ms3a_real_source_payload) (ps : ms3a_sim_source_payload),
+    pr \in d_ms3a_real_source_payload x =>
+    ps \in d_ms3a_sim_source_payload x s =>
+    ms3a_payload_pair_public_fields_match pr ps.
+proof.
+move=> pr ps Hpr Hps; move: Hpr Hps.
+rewrite /d_ms3a_real_source_payload /d_ms3a_sim_source_payload => Hpr Hps.
+case/supp_dmap: Hpr=> [sr [Hsr Heqr]].
+case/supp_dmap: Hps=> [ss [Hss Heqs]].
+have Hm := A_ms3a_seed_pair_public_fields_on_support x s sr ss Hsr Hss.
+by rewrite Heqr Heqs.
+qed.
