docs/03-formal-verification/easycrypt/ms/true_clause/TrueClauseMSB.ec
@@ -1,0 +1,37 @@
+require import AllCore List.
+require import Algebra QssmTypes SchnorrBranch.
+require import TrueClauseTypes.
+
+(* MSB-first strict-greater bit pattern at first differing index + equivalences. *)
+
+pred ms3b_msb_first_strict_gt_at (value_bits target_bits : bool list) (p : int) =
+  ms_bitlists_wf_for_index value_bits target_bits p /\
+  ms_bits_agree_more_significant value_bits target_bits p /\
+  nth witness value_bits p = true /\
+  nth witness target_bits p = false.
+
+lemma L_ms3b_msb_first_strict_gt_at_implies_hdb (vb tb : bool list) (p : int) :
+  ms3b_msb_first_strict_gt_at vb tb p =>
+  ms_highest_differing_bit vb tb p.
+proof.
+move=> Hgt.
+case: Hgt => Hwf [Hag [Hvp Htn]].
+split; first exact Hwf.
+split; first by rewrite Hvp Htn.
+exact Hag.
+qed.
+
+lemma L_ms3b_tcp_iff_msb_first_strict_gt (vb tb : bool list) (p : int) :
+  ms_true_clause_position vb tb p <=> ms3b_msb_first_strict_gt_at vb tb p.
+proof.
+rewrite /ms_true_clause_position /ms3b_msb_first_strict_gt_at /ms_highest_differing_bit.
+split.
+  move=> [Hhd [Htn Hvp]].
+  case: Hhd => Hwf [_ Hag].
+  by split=> //; split=> //; split=> //.
+move=> [Hwf [Hag [Hvp Htn]]].
+split; last by split.
+split; first exact Hwf.
+split; first by rewrite Hvp Htn.
+exact Hag.
+qed.
