docs/03-formal-verification/easycrypt/ms/true_clause/TrueClauseTheorem.ec
@@ -1,0 +1,151 @@
+require import AllCore List.
+require import Algebra QssmTypes SchnorrBranch.
+require import TrueClauseTypes TrueClauseMSB.
+
+(* Semantic axiom, value-bit corollary, and MS_3b_true_clause_characterization chain. *)
+
+axiom A_ms3b_operand_hdb_implies_msb_first_strict_gt :
+  forall (x : ms_public_input) (vb : bool list) (tb : bool list) (p : int),
+    ms3b_comparison_operand_bits x vb tb =>
+    ms_highest_differing_bit vb tb p =>
+    ms3b_msb_first_strict_gt_at vb tb p.
+
+lemma A_ms3b_comparison_semantics :
+  forall (x : ms_public_input) (vb : bool list) (tb : bool list) (p : int),
+    ms3b_comparison_operand_bits x vb tb =>
+    ms_highest_differing_bit vb tb p =>
+    nth witness vb p = true.
+proof.
+move=> x vb tb p Hop Hhd.
+have Hgt := A_ms3b_operand_hdb_implies_msb_first_strict_gt x vb tb p Hop Hhd.
+case: Hgt=> _ [_ [Hvp _]].
+exact Hvp.
+qed.
+
+lemma A_ms3b_hdb_implies_value_one_target_zero :
+  forall (x : ms_public_input) (vb : bool list) (tb : bool list) (p : int),
+    ms3b_comparison_operand_bits x vb tb =>
+    ms_highest_differing_bit vb tb p =>
+    nth witness vb p = true /\
+    nth witness tb p = false.
+proof.
+move=> x vb tb p Hop Hhd.
+have Hvp : nth witness vb p = true by exact (A_ms3b_comparison_semantics x vb tb p Hop Hhd).
+have Hneq : nth witness vb p <> nth witness tb p by exact (A_ms3b_hdb_directionality vb tb p Hhd).
+have Htn : nth witness tb p = false.
+  have Hneq' := Hneq.
+  rewrite Hvp in Hneq'.
+  by case (nth witness tb p) Hneq'.
+split; first exact Hvp.
+exact Htn.
+qed.
+
+lemma A_ms3b_hdb_implies_true_clause_position (vb : bool list) (tb : bool list) (p : int) :
+  ms_highest_differing_bit vb tb p =>
+  nth witness vb p = true =>
+  nth witness tb p = false =>
+  ms_true_clause_position vb tb p.
+proof.
+move=> Hhd Hvp Htn.
+rewrite /ms_true_clause_position.
+split; first exact Hhd.
+split; first exact Htn.
+exact Hvp.
+qed.
+
+lemma A_ms3b_highest_differing_bit_correct :
+  forall (x : ms_public_input) (vb : bool list) (tb : bool list) (p : int),
+    ms3b_comparison_operand_bits x vb tb =>
+    ms_highest_differing_bit vb tb p =>
+    ms_true_clause_position vb tb p.
+proof.
+move=> x vb tb p Hop Hhd.
+have [Hvp Htn] := A_ms3b_hdb_implies_value_one_target_zero x vb tb p Hop Hhd.
+by apply (A_ms3b_hdb_implies_true_clause_position vb tb p Hhd Hvp Htn).
+qed.
+
+lemma A_ms3b_pedersen_opening_correct :
+  forall (x : ms_public_input) (vb : bool list) (tb : bool list) (p : int)
+    (clause_pub : sch_point) (r : scalar),
+    ms3b_clause_opening_binds x vb tb p clause_pub r =>
+    ms_clause_public_point_matches_blinder clause_pub true r.
+proof.
+by move=> x vb tb p clause_pub r Hob; rewrite /ms3b_clause_opening_binds in Hob.
+qed.
+
+lemma MS_3b_bits_from_public_input (x : ms_public_input) (vb : bool list) (tb : bool list) :
+  ms3b_comparison_operand_bits x vb tb =>
+  size vb = size tb /\
+  0 < size vb.
+proof.
+by move=> Hop; apply (A_ms3b_bit_decomposition_correct x vb tb Hop).
+qed.
+
+lemma MS_3b_highest_diff_from_bits (x : ms_public_input) (vb : bool list) (tb : bool list) (p : int) :
+  ms3b_comparison_operand_bits x vb tb =>
+  ms_highest_differing_bit vb tb p =>
+  (size vb = size tb /\ 0 < size vb) /\
+  ms_true_clause_position vb tb p.
+proof.
+move=> Hop Hhd.
+have Hbits := MS_3b_bits_from_public_input x vb tb Hop.
+split; first exact Hbits.
+by apply (A_ms3b_highest_differing_bit_correct x vb tb p Hop Hhd).
+qed.
+
+lemma MS_3b_true_clause_from_highest_diff (x : ms_public_input) (vb : bool list) (tb : bool list) (p : int) :
+  ms3b_comparison_operand_bits x vb tb =>
+  ms_highest_differing_bit vb tb p =>
+  ms_true_clause_position vb tb p.
+proof.
+move=> Hop Hhd.
+have [_ Htcp] := MS_3b_highest_diff_from_bits x vb tb p Hop Hhd.
+by exact Htcp.
+qed.
+
+lemma MS_3b_clause_point_from_opening (x : ms_public_input) (vb : bool list) (tb : bool list) (p : int)
+  (clause_pub : sch_point) (r : scalar) :
+  ms3b_comparison_operand_bits x vb tb =>
+  size vb = size tb /\ 0 < size vb =>
+  ms_true_clause_position vb tb p =>
+  ms3b_clause_opening_binds x vb tb p clause_pub r =>
+  ms_clause_public_point_matches_blinder clause_pub true r.
+proof.
+move=> Hop Hbits Hpos Hob.
+have _ := Hop.
+have _ := Hbits.
+have _ := Hpos.
+exact (A_ms3b_pedersen_opening_correct x vb tb p clause_pub r Hob).
+qed.
+
+lemma MS_3b_true_clause_characterization_from_highest_diff
+  (x : ms_public_input) (vb : bool list) (tb : bool list) (p : int) (clause_pub : sch_point) (r : scalar) :
+  ms3b_comparison_operand_bits x vb tb =>
+  ms_highest_differing_bit vb tb p =>
+  ms_true_clause_position vb tb p =>
+  ms3b_clause_opening_binds x vb tb p clause_pub r =>
+  ms_true_clause_points_are_blinder_points vb tb p clause_pub r.
+proof.
+move=> Hop Hhd Htcp Hob.
+have Hbits := MS_3b_bits_from_public_input x vb tb Hop.
+have Hgeom := MS_3b_highest_diff_from_bits x vb tb p Hop Hhd.
+have Htcl := MS_3b_true_clause_from_highest_diff x vb tb p Hop Hhd.
+have _ := Htcp.
+have _ := Hgeom.
+have _ := Htcl.
+rewrite /ms_true_clause_points_are_blinder_points.
+move=> Hpos.
+exact (MS_3b_clause_point_from_opening x vb tb p clause_pub r Hop Hbits Hpos Hob).
+qed.
+
+lemma MS_3b_true_clause_characterization
+  (x : ms_public_input) (vb : bool list) (tb : bool list) (p : int) (clause_pub : sch_point) (r : scalar) :
+  ms3b_comparison_operand_bits x vb tb =>
+  ms_highest_differing_bit vb tb p =>
+  ms_true_clause_position vb tb p =>
+  ms3b_clause_opening_binds x vb tb p clause_pub r =>
+  ms_true_clause_points_are_blinder_points vb tb p clause_pub r.
+proof.
+move=> Hop Hhd Htcp Hob.
+exact (MS_3b_true_clause_characterization_from_highest_diff x vb tb p clause_pub r Hop Hhd Htcp Hob).
+qed.
