docs/03-formal-verification/easycrypt/ms/true_clause/TrueClauseTypes.ec
@@ -1,0 +1,73 @@
+require import AllCore List.
+require import Algebra QssmTypes SchnorrBranch.
+
+(* MS-3b structural predicates and highest-differing-bit geometry (index 0 = MSB). *)
+
+pred ms3b_comparison_operand_bits
+  (x : ms_public_input) (value_bits target_bits : bool list) =
+  size value_bits = size target_bits /\
+  0 < size value_bits.
+
+pred ms_bitlists_wf_for_index (vb : bool list) (tb : bool list) (p : int) =
+  size vb = size tb /\
+  0 <= p /\
+  p < size vb.
+
+pred ms_bits_agree_more_significant (vb : bool list) (tb : bool list) (p : int) =
+  forall (i : int), 0 <= i => i < p =>
+    nth witness vb i = nth witness tb i.
+
+pred ms_highest_differing_bit (value_bits target_bits : bool list) (p : int) =
+  ms_bitlists_wf_for_index value_bits target_bits p /\
+  nth witness value_bits p <> nth witness target_bits p /\
+  ms_bits_agree_more_significant value_bits target_bits p.
+
+pred ms_true_clause_position (value_bits target_bits : bool list) (p : int) =
+  ms_highest_differing_bit value_bits target_bits p /\
+  nth witness target_bits p = false /\
+  nth witness value_bits p = true.
+
+pred ms_clause_public_point_matches_blinder
+  (commitment : sch_point) (expected_bit : bool) (blinder : scalar) =
+  commitment = sch_pubkey blinder.
+
+pred ms3b_clause_opening_binds
+  (x : ms_public_input) (value_bits target_bits : bool list) (p : int)
+  (clause_pub : sch_point) (r : scalar) =
+  ms_clause_public_point_matches_blinder clause_pub true r.
+
+pred ms_true_clause_points_are_blinder_points
+  (value_bits target_bits : bool list) (p : int)
+  (clause_pub : sch_point) (r : scalar) =
+  ms_true_clause_position value_bits target_bits p =>
+  ms_clause_public_point_matches_blinder clause_pub true r.
+
+lemma A_ms3b_bit_decomposition_correct :
+  forall (x : ms_public_input) (vb : bool list) (tb : bool list),
+    ms3b_comparison_operand_bits x vb tb =>
+    size vb = size tb /\
+    0 < size vb.
+proof.
+by move=> x vb tb [Hsz Hpos]; split=> //.
+qed.
+
+lemma A_ms3b_hdb_implies_bits_above_equal (vb : bool list) (tb : bool list) (p : int) :
+  ms_highest_differing_bit vb tb p =>
+  ms_bits_agree_more_significant vb tb p.
+proof.
+by move=> Hhd; case: Hhd => _ [_ Hag]; exact Hag.
+qed.
+
+lemma A_ms3b_hdb_implies_bitlists_wf (vb : bool list) (tb : bool list) (p : int) :
+  ms_highest_differing_bit vb tb p =>
+  ms_bitlists_wf_for_index vb tb p.
+proof.
+by move=> Hhd; case: Hhd => Hwf _; exact Hwf.
+qed.
+
+lemma A_ms3b_hdb_directionality (vb : bool list) (tb : bool list) (p : int) :
+  ms_highest_differing_bit vb tb p =>
+  nth witness vb p <> nth witness tb p.
+proof.
+by move=> Hhd; case: Hhd => _ [Hneq _]; exact Hneq.
+qed.
